add basic byte parsers

PrimParser/Byte.lean
@@ -1,5 +1,7 @@
 import PrimParser.Basic
 
+open Buffer
+
 /-!
 # Byte parsers
 -/
@@ -7,5 +9,128 @@ import PrimParser.Basic
 namespace Parser
 
 abbrev ByteParser (ε : Type) (g : Grade) (α : Type) : Type := Parser ByteArray UInt8 ε g α
+
+variable
+  {α ε : Type}
+  {n : Nat}
+  {g : Grade}
+  {ge gc : Necessity}
+
+def runBytes (p : ByteParser ε g α) (b : ByteArray) : Except ε α :=
+  p.runOn (Input.ofByteArray b)
+
+def runBytesOption (p : ByteParser ε ⟨ge, gc⟩ α) (b : ByteArray) : Option α :=
+  (p.runBytes b).toOption
+
+namespace Byte
+
+-- TODO csimp
+/-- Consume exactly `k + 1` bytes. -/
+def take1 (k : Nat) : ByteParser Error conditional ByteArray where
+  run {n} t :=
+    if h : k < n then
+      success { result := t.buf.extract t.pos (t.pos + k + 1)
+                restSize := n - (k + 1) }
+    else
+      failure { error := Error.eof
+                restSize := n }
+
+/-- Consume all remaining input. -/
+def takeRest : ByteParser Error flexible ByteArray :=
+  List.toByteArray <$>ᵍ many anyTok
+
+private def takeRestImpl : ByteParser Error flexible ByteArray where
+  run {n} t :=
+    success { result := t.buf.extract t.pos t.buf.size
+              restSize := 0 }
+
+private theorem nextTok_eq (t : Input ByteArray UInt8 (n + 1))
+  (h : t.pos < t.buf.size := by have := t.valid; simp only [Input.pos, size_uint8] at this ⊢; omega)
+  : t.nextTok = some t.buf[t.pos] := by simp [Input.pos]
+
+theorem many_go_anyTok_restSize (n : Nat)
+  : ∀ t : Input ByteArray UInt8 n, (many.go anyTok t).restSize = 0 := by
+  induction n with
+  | zero => intro t; rw [many.go, anyTok_run_eof]
+  | succ n ih => intro t; rw [many.go, anyTok_run_some (nextTok_eq t)]; exact ih _
+
+theorem many_go_anyTok_result (n : Nat)
+  : ∀ t : Input ByteArray UInt8 n, (many.go anyTok t).result = t.buf.data.toList.drop t.pos := by
+  induction n with
+  | zero => intro t; rw [many.go, anyTok_run_eof]; simp [Input.pos]
+  | succ n ih =>
+    intro t
+    have hv : n + 1 ≤ t.buf.size := by simpa using t.valid
+    rw [many.go, anyTok_run_some (nextTok_eq t)]
+    simp only [ih, Input.dropTo, width_uint8, Input.pos, ByteArray.getElem_eq_getElem_data,
+      ← Array.getElem_toList, show t.buf.size - n = t.buf.size - (n + 1) + 1 by omega,
+      List.getElem_cons_drop]
+
+@[csimp] private theorem takeRest_eq_impl : @takeRest = @takeRestImpl := by
+  ext n t
+  simp [takeRest, takeRestImpl, many, GradedFunctor.gmap, Functor.map,
+        many_go_anyTok_result, many_go_anyTok_restSize, ByteArray.ext_iff, List.toArray_drop]
+
+/-- Read an unsigned 8-bit integer. -/
+abbrev uint8 : ByteParser Error conditional UInt8 := anyTok
+
+/-- Read a signed 8-bit integer. -/
+def int8 : ByteParser Error conditional Int8 := (·.toInt8) <$>ᵍ uint8
+
+/-- Read a big-endian unsigned 16-bit integer. -/
+def uint16be : ByteParser Error conditional UInt16 := gdo
+  let hi ← uint8
+  let lo ← uint8
+  return hi.toUInt16 <<< 8 ||| lo.toUInt16
+
+/-- Read a little-endian unsigned 16-bit integer. -/
+def uint16le : ByteParser Error conditional UInt16 := gdo
+  let lo ← uint8
+  let hi ← uint8
+  return hi.toUInt16 <<< 8 ||| lo.toUInt16
+
+/-- Read a big-endian unsigned 32-bit integer. -/
+def uint32be : ByteParser Error conditional UInt32 := gdo
+  let hi ← uint16be
+  let lo ← uint16be
+  return hi.toUInt32 <<< 16 ||| lo.toUInt32
+
+/-- Read a little-endian unsigned 32-bit integer. -/
+def uint32le : ByteParser Error conditional UInt32 := gdo
+  let lo ← uint16le
+  let hi ← uint16le
+  return hi.toUInt32 <<< 16 ||| lo.toUInt32
+
+/-- Read a big-endian unsigned 64-bit integer. -/
+def uint64be : ByteParser Error conditional UInt64 := gdo
+  let hi ← uint32be
+  let lo ← uint32be
+  return hi.toUInt64 <<< 32 ||| lo.toUInt64
+
+/-- Read a little-endian unsigned 64-bit integer. -/
+def uint64le : ByteParser Error conditional UInt64 := gdo
+  let lo ← uint32le
+  let hi ← uint32le
+  return hi.toUInt64 <<< 32 ||| lo.toUInt64
+
+/-- Read a big-endian signed 16-bit integer. -/
+def int16be : ByteParser Error conditional Int16 := (·.toInt16) <$>ᵍ uint16be
+
+/-- Read a little-endian signed 16-bit integer. -/
+def int16le : ByteParser Error conditional Int16 := (·.toInt16) <$>ᵍ uint16le
+
+/-- Read a big-endian signed 32-bit integer. -/
+def int32be : ByteParser Error conditional Int32 := (·.toInt32) <$>ᵍ uint32be
+
+/-- Read a little-endian signed 32-bit integer. -/
+def int32le : ByteParser Error conditional Int32 := (·.toInt32) <$>ᵍ uint32le
+
+/-- Read a big-endian signed 64-bit integer. -/
+def int64be : ByteParser Error conditional Int64 := (·.toInt64) <$>ᵍ uint64be
+
+/-- Read a little-endian signed 64-bit integer. -/
+def int64le : ByteParser Error conditional Int64 := (·.toInt64) <$>ᵍ uint64le
+
+end Byte
 
 end Parser
